Impl/CommitterImpl.i.dfy
@@ -1222,8 +1222,10 @@ module CommitterImpl {
 
     ensures old_self.ReadSuperblockResp(IIO(io), which) == self
     {
-      var id, sector := IOImpl.ReadSector(io);
-      var res := (if sector.Some? && sector.value.SectorSuperblock?
+      var id;
+      linear var sector;
+      id, sector := IOImpl.ReadSector(io);
+      var res := (if sector.lSome? && sector.value.SectorSuperblock?
           then JC.SuperblockSuccess(sector.value.superblock)
           else JC.SuperblockCorruption);
       if which == 0 {
@@ -1240,6 +1242,10 @@ module CommitterImpl {
         } else {
           print "readSuperblockResp did nothing\n";
         }
+      }
+      linear match sector {
+        case lSome(value) => value.Free();
+        case lNone() => {}
       }
 
       IOModel.ReadSectorCorrect(IIO(io));
