Impl/SuccImpl.i.dfy
@@ -16,7 +16,8 @@ module SuccImpl {
   import opened StateBCImpl
   import opened BucketImpl
   import opened Lexicographic_Byte_Order_Impl
-  import opened BoxNodeImpl
+  import opened NodeImpl
+  import CacheImpl
 
   import BGI = BucketGeneratorImpl
   import BGM = BucketGeneratorModel
@@ -39,28 +40,30 @@ module SuccImpl {
   import opened BucketsLib
   import opened BoundedPivotsLib
 
-  import opened PBS = PivotBetreeSpec`Spec
-
-  method composeGenerator(node: Node, r: uint64, linear g: lOption<BGI.Generator>, ghost acc: seq<Bucket>, ghost bucket: Bucket, start: UI.RangeStart) returns (linear g': BGI.Generator)
-  requires node.Inv()
-  requires r as nat < |node.Read().buckets|
-  requires bucket == node.Read().buckets[r as nat].I()
-  requires SSM.WFNode(node.I())
+  method composeGenerator(cache: CacheImpl.MutCache, ref: BT.G.Reference, r: uint64, 
+    linear g: lOption<BGI.Generator>, ghost acc: seq<Bucket>, ghost bucket: Bucket,
+    start: UI.RangeStart)
+  returns (linear g': BGI.Generator)
+  requires cache.Inv()
+  requires cache.ptr(ref).Some?
+  requires SSM.WFNode(cache.I()[ref])
+  requires r as nat < |cache.I()[ref].buckets|
+  requires bucket == cache.I()[ref].buckets[r as nat]
   requires WFBucket(bucket)
   requires forall i | 0 <= i < |acc| :: WFBucket(acc[i])
   requires g.lSome? <==> |acc| >= 1
-  requires g.lSome? ==> g.value.Inv() && g.value.I() == BGM.GenFromBucketStackWithLowerBound(acc, start)
-  ensures g'.Inv() && g'.I() == BGM.GenFromBucketStackWithLowerBound(acc + [bucket], start);
+  requires g.lSome? ==> g.value.Inv() && g.value.I()
+    == BGM.GenFromBucketStackWithLowerBound(acc, start)
+  ensures g'.Inv() && g'.I()
+    == BGM.GenFromBucketStackWithLowerBound(acc + [bucket], start)
   {
-    linear var g2 := BGI.Generator.GenFromBucketWithLowerBound(lseq_peek(node.box.Borrow().buckets, r), start);
+    linear var g2 := cache.NodeBucketGen(ref, r, start);
     BGM.reveal_GenFromBucketStackWithLowerBound();
     linear match g {
       case lSome(g1) =>
         g' := BGI.Generator.GenCompose(g1, g2);
-        assert g'.Inv() && g'.I() == BGM.GenFromBucketStackWithLowerBound(acc + [bucket], start);
       case lNone() => 
         g' := g2;
-        assert g'.Inv() && g'.I() == BGM.GenFromBucketStackWithLowerBound([bucket], start);
     }
   }
 
@@ -75,36 +78,39 @@ module SuccImpl {
       maxToFind: uint64,
       ref: BT.G.Reference,
       counter: uint64,
-      node: Node)
+      pivots: PivotTable,
+      children: Option<seq<BT.G.Reference>>)
   returns (res : Option<UI.SuccResultList>)
-  requires Inv(s)
-  requires node.Inv()
-  requires SSM.WFNode(node.I())
   requires s.ready
+  requires Inv(s)
   requires io.initialized()
-  requires ref in s.I().cache
+  requires s.cache.ptr(ref).Some?
+  requires SSM.WFNode(s.cache.I()[ref])
+  requires pivots == s.cache.I()[ref].pivotTable
+  requires children == s.cache.I()[ref].children
+  requires BoundedKey(pivots, key)
   requires ref in s.I().ephemeralIndirectionTable.graph
-  requires node.I() == s.I().cache[ref]
   requires maxToFind >= 1
   requires |acc| + counter as int < 0x1_0000_0000_0000_0000 - 1
   requires forall i | 0 <= i < |acc| :: WFBucket(acc[i])
   requires g.lSome? <==> |acc| >= 1
-  requires g.lSome? ==> g.value.Inv() && g.value.I() == BGM.GenFromBucketStackWithLowerBound(acc, start)
+  requires g.lSome? ==> g.value.Inv() && g.value.I()
+    == BGM.GenFromBucketStackWithLowerBound(acc, start)
   requires io !in s.Repr()
-  requires BoundedKey(node.I().pivotTable, key)
   modifies s.Repr()
   modifies io
   decreases counter, 0
   ensures WellUpdated(s)
+  ensures s.cache.I() == old(s.cache.I())
   ensures (s.I(), IIO(io), res)
-       == SuccModel.getPathInternal(old(s.I()), old(IIO(io)), key, old(acc), start, upTo, maxToFind as int, ref, counter, old(node.I()))
+       == SuccModel.getPathInternal(old(s.I()), old(IIO(io)), key, old(acc),
+      start, upTo, maxToFind as int, ref, counter, s.cache.I()[ref])
   {
     SuccModel.reveal_getPathInternal();
 
-    var pivots := node.GetPivots();
     var r := Pivots.ComputeRoute(pivots, key);
-
-    ghost var bucket := node.Read().buckets[r as nat].I();
+    ghost var node := s.cache.I()[ref];
+    ghost var bucket := s.cache.I()[ref].buckets[r as nat];
     ghost var acc' := acc + [bucket];
 
     var upTo';
@@ -121,7 +127,6 @@ module SuccImpl {
       }
     }
 
-    var children := node.GetChildren();
     if children.Some? {
       if counter == 0 {
         print "getPathInternal failure: count ran down\n";
@@ -133,21 +138,27 @@ module SuccImpl {
         }
 
         assert (s.I(), IIO(io), res)
-         == SuccModel.getPathInternal(old(s.I()), old(IIO(io)), key, old(acc), start, upTo, maxToFind as int, ref, counter, old(node.I()));
+         == SuccModel.getPathInternal(old(s.I()), old(IIO(io)), key, old(acc),
+          start, upTo, maxToFind as int, ref, counter, node);
       } else {
-        BookkeepingModel.lemmaChildInGraph(s.I(), ref, node.I().children.value[r]);
-        linear var g' := composeGenerator(node, r, g, acc, bucket, start);
-        res := getPath(s, io, key, acc', lSome(g'), start, upTo', maxToFind, children.value[r], counter - 1);
-
+        BookkeepingModel.lemmaChildInGraph(s.I(), ref, children.value[r]);
+        linear var g' := composeGenerator(s.cache, ref, r, g, acc, bucket, start);
+        res := getPath(s, io, key, acc', lSome(g'), start, upTo', maxToFind,
+          children.value[r], counter - 1);
+        
         assert (s.I(), IIO(io), res)
-         == SuccModel.getPathInternal(old(s.I()), old(IIO(io)), key, old(acc), start, upTo, maxToFind as int, ref, counter, old(node.I()));
+         == SuccModel.getPathInternal(old(s.I()), old(IIO(io)), key, old(acc),
+          start, upTo, maxToFind as int, ref, counter, node);
       }
     } else {
-      linear var g' := composeGenerator(node, r, g, acc, bucket, start);
-      var res0 := BucketSuccessorLoopImpl.GetSuccessorInBucketStack(g', acc', maxToFind, start, upTo');
+      linear var g' := composeGenerator(s.cache, ref, r, g, acc, bucket, start);
+      var res0 := BucketSuccessorLoopImpl.GetSuccessorInBucketStack(g', acc',
+        maxToFind, start, upTo');
       res := Some(res0);
+
       assert (s.I(), IIO(io), res)
-       == SuccModel.getPathInternal(old(s.I()), old(IIO(io)), key, old(acc), start, upTo, maxToFind as int, ref, counter, old(node.I()));
+       == SuccModel.getPathInternal(old(s.I()), old(IIO(io)), key,
+        old(acc), start, upTo, maxToFind as int, ref, counter, node);
     }
   }
 
@@ -172,25 +183,25 @@ module SuccImpl {
   requires io !in s.Repr()
   requires |acc| + counter as int < 0x1_0000_0000_0000_0000 - 1
   requires g.lSome? <==> |acc| >= 1
-  requires g.lSome? ==> g.value.Inv() && g.value.I() == BGM.GenFromBucketStackWithLowerBound(acc, start)
+  requires g.lSome? ==> g.value.Inv() && g.value.I()
+    == BGM.GenFromBucketStackWithLowerBound(acc, start)
   modifies s.Repr()
   modifies io
   decreases counter, 1
   ensures WellUpdated(s)
   ensures (s.I(), IIO(io), res)
-       == SuccModel.getPath(old(s.I()), old(IIO(io)), key, old(acc), start, upTo, maxToFind as int, ref, counter)
+       == SuccModel.getPath(old(s.I()), old(IIO(io)), key, old(acc), start,
+        upTo, maxToFind as int, ref, counter)
   {
     SuccModel.reveal_getPath();
 
-    var nodeOpt := s.cache.GetOpt(ref);
-    if nodeOpt.Some? {
-      var node := nodeOpt.value;
-
-      assert node.I() == s.I().cache[ref];
-      var pivots := node.GetPivots();
+    var incache := s.cache.InCache(ref);
+    if incache {
+      var pivots, children := s.cache.GetNodeInfo(ref);
       var boundedkey := ComputeBoundedKey(pivots, key);
       if boundedkey {
-        res := getPathInternal(s, io, key, acc, g, start, upTo, maxToFind, ref, counter, node);
+        res := getPathInternal(s, io, key, acc, g, start, upTo,
+          maxToFind, ref, counter, pivots, children);
         LruModel.LruUse(s.I().lru, ref);
         s.lru.Use(ref);
       } else {
@@ -229,7 +240,8 @@ module SuccImpl {
   modifies io
   modifies s.Repr()
   ensures WellUpdated(s)
-  ensures (s.I(), IIO(io), res) == SuccModel.doSucc(old(s.I()), old(IIO(io)), start, maxToFind as int)
+  ensures (s.I(), IIO(io), res) == SuccModel.doSucc(old(s.I()), old(IIO(io)),
+    start, maxToFind as int)
   {
     SuccModel.reveal_doSucc();
     var startKey := if start.NegativeInf? then [] else start.key;
