lib/DataStructures/LinearContentMutableMap.i.dfy
@@ -1,0 +1,734 @@
+include "../Lang/LinearSequence.s.dfy"
+include "../Lang/LinearSequence.i.dfy"
+include "../Base/LinearOption.i.dfy"
+include "../Lang/Inout.i.dfy"
+
+include "../Lang/NativeTypes.s.dfy"
+include "../Base/Option.s.dfy"
+include "../Base/sequences.i.dfy"
+include "../Base/Sets.i.dfy"
+include "../Base/Maps.i.dfy"
+include "LinearMutableMapBase.i.dfy"
+
+//
+// Immutable (functional) model to support MutableMapImpl.  API provides an
+// iterator interface with a deterministic order for parsing/marshaling.
+// (That's why the API is/ more than just a Dafny map.)
+//
+// TODO(jonh): Here and elsewhere, Model files seem to be both
+// API (because callers use some of the definitions as 'public' ways
+// to reason about the behavior of the modeled Impl) and internal
+// proof (the logic half of the behavior of the Impl). It would be
+// nice to cleanly separate these concerns.
+//
+
+module LinearContentMutableMap {
+  import opened NativeTypes
+  import opened Options
+  import opened LinearOption
+  import opened Sequences
+  import opened Sets
+  import opened Maps
+
+  import opened LinearSequence_i
+  import opened LinearSequence_s
+  import opened Inout
+  import opened Base = LinearMutableMapBase
+
+  linear datatype lItem<V> = Empty | Entry(key: uint64, linear value: V) | Tombstone(key: uint64)
+  {
+    linear method FreeNonEntry()
+    requires !this.Entry? 
+    {
+      linear match this {
+        case Empty() => 
+        case Tombstone(key) =>
+      }
+    }
+
+    function toItem(): Item<V>
+    {
+      match this {
+        case Empty() => Base.Empty()
+        case Entry(key, value) => Base.Entry(key, value)
+        case Tombstone(key) => Base.Tombstone(key)
+      }
+    }
+  }
+
+  function toItems<V>(litems: lseq<lItem<V>>): (items: seq<Item<V>>)
+  ensures |items| == |litems|
+  {
+    var elements := lseqs(litems);
+    seq (|elements|, i requires 0 <= i < |elements| => elements[i].toItem())
+  }
+
+  linear datatype FixedSizeLinearHashMap<V> = FixedSizeLinearHashMap(
+    linear storage: lseq<lItem<V>>,
+    count: uint64,
+    ghost contents: map<uint64, Option<V>>)
+
+  function method Uint64SlotForKey<V>(shared self: FixedSizeLinearHashMap<V>, key: uint64): (result: uint64)
+  requires 0 < |self.storage| < 0x1_0000_0000_0000_0000
+  ensures ValidSlot(|self.storage|, Slot(result as nat))
+  ensures Slot(result as nat) == SlotForKey(|self.storage|, key)
+  {
+    var h := hash64(key);
+    var storageLength := lseq_length_as_uint64(self.storage);
+    h % (storageLength as uint64)
+  }
+
+  predicate FixedSizeInv<V>(self: FixedSizeLinearHashMap<V>)
+  {
+    && 128 <= |self.storage| < 0x1_0000_0000_0000_0000
+    && (self.count as nat) < 0x1_0000_0000_0000_0000
+    && self.count as nat < |self.storage|
+
+    && |self.contents| == (self.count as nat)
+    && lseq_has_all(self.storage)
+    && SeqMatchesContentKeys(toItems(self.storage), self.contents)
+    && EntriesMatchContentValue(toItems(self.storage), self.contents)
+    && TombstonesMatchContentValue(toItems(self.storage), self.contents)
+  }
+
+  predicate IsConstructorFromSize<V>(size: nat, self: FixedSizeLinearHashMap<V>)  
+  {
+    && |self.storage| == size
+    && self.count == 0
+    && self.contents == map[]
+    && (forall slot :: ValidSlot(|self.storage|, slot) ==> SlotIsEmpty(toItems(self.storage), slot))
+    && FixedSizeInv(self)
+  }
+
+  method ConstructorFromSize<V>(size: uint64) returns (linear self: FixedSizeLinearHashMap<V>)
+  requires 128 <= size
+  ensures IsConstructorFromSize(size as nat, self)
+  {
+    linear var storage := lseq_alloc(size);
+
+    var i := 0 as uint64;
+    while i < size
+      invariant i <= size
+      invariant size as nat == |storage|
+      invariant forall j | 0 <= j < i as nat :: lseq_has(storage)[j]
+      invariant forall j | i as nat <= j < size as nat :: !lseq_has(storage)[j]
+      invariant forall slot :: ValidSlot(|storage|, slot) && 0 <= slot.slot < i as nat 
+          ==> SlotIsEmpty(toItems(storage), slot)
+    {
+      linear var item := lItem.Empty();
+      lseq_give_inout(inout storage, i, item);
+      i := i + 1;
+    }
+
+    self := FixedSizeLinearHashMap(
+     /* storage := */ storage,
+     /* count := */ 0,
+     /* contents := */ map[]);
+  }
+
+  lemma allNonEmptyImpliesCountEqStorageSize<V>(self: FixedSizeLinearHashMap<V>)
+  requires FixedSizeInv(self)
+  ensures (forall j | 0 <= j < |self.storage| :: !self.storage[j].Empty?)
+      ==> self.count as int == |self.storage|
+  {
+    var elements := self.storage;
+    if forall j | 0 <= j < |elements| :: !elements[j].Empty? {
+      var elementIndices := set i | 0 <= i < |elements|;
+      assert IndexSetThrough(toItems(elements), |elements|) == elementIndices; // trigger
+      CardinalityOfSetsOfSequenceIndices(toItems(elements), elementIndices);
+      IndexSetMatchesContents(toItems(elements), self.contents);
+    }
+  }
+
+  function {:opaque} getEmptyWitness<V>(self: FixedSizeLinearHashMap<V>, i: uint64) : (res : uint64)
+  requires FixedSizeInv(self)
+  requires 0 <= i as int <= |self.storage|
+  requires forall j | 0 <= j < i as int :: !self.storage[j].Empty?
+  requires self.count as int < |self.storage|
+  decreases |self.storage| - i as int
+  ensures 0 <= res as int < |self.storage|
+  ensures self.storage[res as int].Empty?
+  {
+    allNonEmptyImpliesCountEqStorageSize(self);
+
+    if self.storage[i as int].Empty? then
+      i
+    else
+      getEmptyWitness(self, i+1)
+  }
+
+  method Probe<V>(shared self: FixedSizeLinearHashMap<V>, key: uint64)
+  returns (slotIdx: uint64, ghost startSlotIdx: uint64, ghost skips: uint64)
+  requires FixedSizeInv(self)
+  requires self.count as int < |self.storage|
+  ensures 0 <= slotIdx as int < |self.storage|
+  ensures ValidSlot(|self.storage|, Slot(slotIdx as nat))
+  ensures ValidSlot(|self.storage|, Slot(startSlotIdx as nat))
+  ensures Slot(startSlotIdx as nat) == SlotForKey(|self.storage|, key)
+  ensures 0 <= skips
+  ensures slotIdx as nat == KthSlotSuccessor(|self.storage|, Slot(startSlotIdx as nat), skips as nat).slot
+  ensures key in self.contents ==> SlotExplainsKey(toItems(self.storage), skips as nat, key)
+  ensures key !in self.contents ==> FilledWithOtherKeys(toItems(self.storage), Slot(startSlotIdx as nat), skips as nat, key) && (self.storage[slotIdx as nat].Empty? || (self.storage[slotIdx as nat].Tombstone? && self.storage[slotIdx as nat].key == key))
+  ensures self.storage[slotIdx as nat].Entry? ==> key in self.contents && key == self.storage[slotIdx as nat].key
+  ensures self.storage[slotIdx as nat].Empty? ==> key !in self.contents
+  {
+    slotIdx := Uint64SlotForKey(self, key);
+    startSlotIdx := slotIdx;
+    ghost var startSlot := Slot(startSlotIdx as nat);
+
+    ghost var viewFromStartSlot := View(toItems(self.storage), startSlotIdx as nat);
+    ViewsHaveConsistentCounts(toItems(self.storage), viewFromStartSlot, startSlotIdx as nat);
+    CountFilledMatchesIndexSet(toItems(self.storage));
+    IndexSetMatchesContents(toItems(self.storage), self.contents);
+
+    forall dist: nat | dist < |self.storage|
+    ensures self.storage[KthSlotSuccessor(|self.storage|, startSlot, dist).slot].toItem() == viewFromStartSlot[dist]
+    {
+      KthSlotSuccessorWrapsAround(|self.storage|, startSlot, dist); // observe
+    }
+
+    skips := 0;
+
+    while true
+    invariant skips < (|self.storage| as uint64)
+    invariant slotIdx < (|self.storage| as uint64)
+    invariant |self.storage| == |viewFromStartSlot|
+    invariant toItems(self.storage)[startSlotIdx..] + toItems(self.storage)[..startSlotIdx] == viewFromStartSlot
+    invariant slotIdx as nat == KthSlotSuccessor(|self.storage|, startSlot, skips as nat).slot
+    invariant skips < (|self.storage| as uint64) ==> self.storage[slotIdx as nat].toItem() == viewFromStartSlot[skips]
+    invariant ValidSlot(|self.storage|, KthSlotSuccessor(|self.storage|, startSlot, skips as nat))
+    invariant FilledWithOtherKeys(toItems(self.storage), startSlot, skips as nat, key)
+    invariant CountFilled(viewFromStartSlot[..skips]) == skips as nat
+    decreases var wit := getEmptyWitness(self, 0);
+      if slotIdx > wit
+        then wit as int - slotIdx as int + |self.storage|
+        else wit as int - slotIdx as int
+    {
+      ghost var skipsBefore := skips;
+      shared var entry := lseq_peek(self.storage, slotIdx);
+      if entry.Empty? || (entry.Tombstone? && entry.key == key) {
+        assert key in self.contents ==> SlotExplainsKey(toItems(self.storage), skips as nat, key) by {
+          reveal_SomeSkipCountExplainsKey();
+        }
+        return;
+      } else if entry.key == key {
+        assert EntryInSlotMatchesContents(toItems(self.storage), Slot(slotIdx as nat), self.contents); // observe
+        return;
+      }
+
+      // -- increment --
+      slotIdx := Uint64SlotSuccessorUint64(lseq_length_as_uint64(self.storage), slotIdx);
+      skips := skips + 1;
+      // ---------------
+
+      assert viewFromStartSlot[..skips] == viewFromStartSlot[..skipsBefore] + [viewFromStartSlot[skipsBefore]]; // observe
+      CountFilledAdditive(viewFromStartSlot[..skipsBefore], [viewFromStartSlot[skipsBefore]]);
+      if skips == |self.storage| as uint64 {
+        forall ensures false
+        {
+          calc {
+            |self.storage|;
+            skips as nat;
+            CountFilled(viewFromStartSlot[..skips]);
+              { assert viewFromStartSlot[..skips] == viewFromStartSlot; } // observe
+            CountFilled(viewFromStartSlot);
+            |self.contents|;
+            self.count as nat;
+            < |self.storage|;
+          }
+        }
+      }
+    }
+  }
+
+  method FixedSizeInsert<V>(linear inout self: FixedSizeLinearHashMap, key: uint64, linear value: V)
+  returns (linear replaced: lOption<V>)
+  requires FixedSizeInv(old_self)
+  requires old_self.count as nat < |old_self.storage| - 1
+  ensures FixedSizeInv(self)
+  ensures self.contents == old_self.contents[key := Some(value)]
+  ensures key !in old_self.contents ==> replaced.lNone?
+  ensures key in old_self.contents ==> replaced.Option() == old_self.contents[key]
+  ensures replaced.lSome? ==> key in old_self.contents
+  ensures |self.storage| == |old_self.storage|
+  {
+    linear var entry := lItem.Entry(key, value);
+    replaced := FixedSizeInsertEntry(inout self, entry);
+  }
+
+  method FixedSizeInsertEntry<V>(linear inout self: FixedSizeLinearHashMap, linear entry: lItem<V>)
+  returns (linear replaced: lOption<V>)
+  requires entry.Entry?
+  requires FixedSizeInv(old_self)
+  requires old_self.count as nat < |old_self.storage| - 1
+  ensures FixedSizeInv(self)
+  ensures self.contents == old_self.contents[entry.key := Some(entry.value)]
+  ensures entry.key !in old_self.contents ==> replaced.lNone?
+  ensures entry.key in old_self.contents ==> replaced.Option() == old_self.contents[entry.key]
+  ensures replaced.lSome? ==> entry.key in old_self.contents
+  ensures |self.storage| == |old_self.storage|
+  {
+    var slotIdx;
+    ghost var probeStartSlotIdx, probeSkips;
+    slotIdx, probeStartSlotIdx, probeSkips := Probe(self, entry.key);
+
+    ghost var contents := old_self.contents[entry.key := Some(entry.value)];
+    inout ghost self.contents := contents;
+    
+    linear var olditem := lseq_take_inout(inout self.storage, slotIdx);
+    lseq_give_inout(inout self.storage, slotIdx, entry);
+
+    if olditem.Empty? {
+      olditem.FreeNonEntry();
+      inout self.count := self.count + 1;
+      replaced := lNone;
+   } else if olditem.Tombstone? {
+      olditem.FreeNonEntry();
+      replaced := lNone;
+    } else {
+      linear var Entry(_, value) := olditem;
+      replaced := lSome(value);
+    }
+
+    forall explainedKey | explainedKey in self.contents
+    ensures exists skips :: SlotExplainsKey(toItems(self.storage), skips, explainedKey)
+    {
+      if entry.key == explainedKey {
+        assert SlotExplainsKey(toItems(self.storage), probeSkips as nat, entry.key); // observe
+      } else {
+        var oldSkips :| SlotExplainsKey(toItems(old_self.storage), oldSkips, explainedKey);
+        assert SlotExplainsKey(toItems(self.storage), oldSkips, explainedKey); // observe
+      }
+    }
+  
+    forall slot | ValidSlot(|self.storage|, slot) && toItems(self.storage)[slot.slot].Entry?
+    ensures && var item := toItems(self.storage)[slot.slot];
+            && self.contents[item.key] == Some(item.value)
+    {
+      var item := toItems(self.storage)[slot.slot];
+      if slot != Slot(slotIdx as nat) {
+        if item.key == entry.key {
+          assert TwoNonEmptyValidSlotsWithSameKey(toItems(self.storage), slot, Slot(slotIdx as nat)); // observe
+          assert SameSlot(|self.storage|, slot, Slot(slotIdx as nat)); // observe
+          assert false;
+        }
+      }
+    }
+
+    forall slot | ValidSlot(|self.storage|, slot) && toItems(self.storage)[slot.slot].Tombstone?
+    ensures && var item := self.storage[slot.slot];
+            && self.contents[item.key].None?
+    {
+      var item := self.storage[slot.slot];
+      if slot != Slot(slotIdx as nat) {
+        if item.key == entry.key {
+          assert TwoNonEmptyValidSlotsWithSameKey(toItems(self.storage), slot, Slot(slotIdx as nat)); // observe
+          assert SameSlot(|self.storage|, slot, Slot(slotIdx as nat)); // observe
+          assert false;
+        }
+      }
+    }
+  }
+
+  method FixedSizeUpdateBySlot<V>(linear inout self: FixedSizeLinearHashMap<V>, slotIdx: uint64, linear value: V)
+  returns (linear replaced: V)
+  requires FixedSizeInv(old_self)
+  requires 0 <= slotIdx as int < |old_self.storage|
+  requires old_self.storage[slotIdx as nat].Entry?
+  ensures FixedSizeInv(self)
+  {
+    linear var entry: lItem<V> := lseq_take_inout(inout self.storage, slotIdx);
+    linear var Entry(key, oldvalue) := entry;
+    lseq_give_inout(inout self.storage, slotIdx, lItem.Entry(key, value));
+    replaced := oldvalue;
+
+    inout ghost self.contents := self.contents[key := Some(value)];
+    assert EntryInSlotMatchesContents(toItems(old_self.storage), Slot(slotIdx as int), old_self.contents);
+
+    forall explainedKey | explainedKey in self.contents
+    ensures exists skips :: SlotExplainsKey(toItems(self.storage), skips, explainedKey)
+    {
+      var oldSkips :| SlotExplainsKey(toItems(old_self.storage), oldSkips, explainedKey);
+      assert SlotExplainsKey(toItems(self.storage), oldSkips, explainedKey); // observe
+    }
+  
+    forall slot | ValidSlot(|self.storage|, slot)
+        && SlotIsEntry(toItems(self.storage), slot)
+    ensures EntryInSlotMatchesContents(toItems(self.storage), slot, self.contents)
+    {
+      assert EntryInSlotMatchesContents(toItems(old_self.storage), slot, old_self.contents);
+      if old_self.storage[slot.slot].key == key {
+        assert TwoNonEmptyValidSlotsWithSameKey(toItems(old_self.storage), slot, Slot(slotIdx as int));
+      }
+    }
+
+    forall slot | ValidSlot(|self.storage|, slot)
+        && toItems(self.storage)[slot.slot].Tombstone?
+    ensures TombstoneInSlotMatchesContents(toItems(self.storage), slot, self.contents)
+    {
+      if slot.slot != slotIdx as nat && old_self.storage[slot.slot].key == key {
+        assert TwoNonEmptyValidSlotsWithSameKey(toItems(self.storage), slot, Slot(slotIdx as nat)); // observe
+        assert SameSlot(|self.storage|, slot, Slot(slotIdx as nat)); // observe
+        assert false;
+      }
+    }
+  }
+
+  method IsEntry<V>(shared self: FixedSizeLinearHashMap<V>, key: uint64) returns (b: bool)
+  requires FixedSizeInv(self)
+  ensures b == (key in self.contents && self.contents[key].Some?)
+  {
+    var slotIdx, _, _ := Probe(self, key);
+    b := lseq_peek(self.storage, slotIdx).Entry?;
+    assert b == (key in self.contents && self.contents[key].Some?);
+  }
+
+  method FixedSizeGet<V>(shared self: FixedSizeLinearHashMap<V>, key: uint64)
+  returns (shared found: V)
+  requires FixedSizeInv(self)
+  requires key in self.contents && self.contents[key].Some?
+  ensures found == self.contents[key].value
+  {
+    var slotIdx, _, _ := Probe(self, key);
+    found := lseq_peek(self.storage, slotIdx).value;
+    // TODO(Jialin): update to return shared lOption<V>
+  }
+
+  method FixedSizeRemove<V>(linear inout self: FixedSizeLinearHashMap<V>, key: uint64)
+  returns (linear removed: lOption<V>)
+  requires FixedSizeInv(old_self)
+  ensures FixedSizeInv(self)
+  ensures (self.contents == if key in old_self.contents
+    then old_self.contents[key := None]
+    else old_self.contents)
+  ensures (removed == if key in old_self.contents && old_self.contents[key].Some?
+    then lSome(old_self.contents[key].value)
+    else lNone)
+  ensures (removed.lSome? <==> (key in old_self.contents && old_self.contents[key].Some?))
+  ensures (self.count == old_self.count)
+  {
+    var slotIdx;
+    ghost var probeStartSlotIdx, probeSkips;
+    slotIdx, probeStartSlotIdx, probeSkips := Probe(self, key);
+
+    if lseq_peek(self.storage, slotIdx).Entry? {
+      linear var item: lItem<V> := lseq_take_inout(inout self.storage, slotIdx);
+      lseq_give_inout(inout self.storage, slotIdx, lItem.Tombstone(key));
+      linear var Entry(_, value) := item;
+      removed := lSome(value);
+
+      inout ghost self.contents := self.contents[key := None];
+      assert EntryInSlotMatchesContents(toItems(old_self.storage), Slot(slotIdx as int), old_self.contents);
+
+      forall explainedKey | explainedKey in self.contents
+      ensures exists skips :: SlotExplainsKey(toItems(self.storage), skips, explainedKey)
+      {
+        if key == explainedKey {
+          assert SlotExplainsKey(toItems(self.storage), probeSkips as nat, key);
+        } else {
+          var oldSkips :| SlotExplainsKey(toItems(old_self.storage), oldSkips, explainedKey);
+          assert SlotExplainsKey(toItems(self.storage), oldSkips, explainedKey);
+        }
+      }
+
+      forall slot | ValidSlot(|self.storage|, slot) && toItems(self.storage)[slot.slot].Entry?
+      ensures && var item := self.storage[slot.slot];
+              && self.contents[item.key] == Some(item.value)
+      {
+        var item := self.storage[slot.slot];
+        if slot != Slot(slotIdx as nat) && item.key == key {
+          assert CantEquivocateStorageKey(toItems(self.storage));
+          assert TwoNonEmptyValidSlotsWithSameKey(toItems(self.storage), slot, Slot(slotIdx as nat));
+          assert false;
+        }
+      }
+    } else {
+      removed := lNone;
+    }
+  }
+
+  //////// Resizing Hash Map
+
+  linear datatype LinearHashMap<V> = LinearHashMap(
+    linear underlying: FixedSizeLinearHashMap<V>,
+    count: uint64,
+    ghost contents: map<uint64, V>)
+  {
+    predicate Inv() {Inv0(this)} // HACK Inv0: is there a better way to refer to the outer Inv(...) from inside Inv()?
+  }
+
+  lemma CantEquivocateMapFromStorageKey<V>(underlying: FixedSizeLinearHashMap<V>)
+  requires FixedSizeInv(underlying)
+  ensures CantEquivocate(toItems(underlying.storage))
+  {
+    assert |underlying.storage| > 0;
+    assert ValidSlot(|underlying.storage|, Slot(0));
+    assert exists slot :: ValidSlot(|underlying.storage|, slot);
+    forall slot1, slot2 | (
+      && ValidSlot(|underlying.storage|, slot1) && ValidSlot(|underlying.storage|, slot2)
+      && underlying.storage[slot1.slot].Entry? && underlying.storage[slot2.slot].Entry?
+      && underlying.storage[slot1.slot].key == underlying.storage[slot2.slot].key)
+    ensures slot1 == slot2
+    {
+      assert CantEquivocateStorageKey(toItems(underlying.storage));
+      if underlying.storage[slot1.slot].Entry? && underlying.storage[slot2.slot].Entry? &&
+        underlying.storage[slot1.slot].key == underlying.storage[slot2.slot].key {
+
+        assert TwoNonEmptyValidSlotsWithSameKey(toItems(underlying.storage), slot1, slot2);
+        if slot1 != slot2 {
+          assert false;
+        }
+        assert slot1 == slot2;
+      } else {
+        assert slot1 == slot2;
+      }
+    }
+  }
+
+  predicate UnderlyingContentsMatchesContents<V>(underlying: FixedSizeLinearHashMap<V>, contents: map<uint64, V>)
+  {
+    && (forall key :: key in contents ==> key in underlying.contents && underlying.contents[key] == Some(contents[key]))
+    && (forall key :: key !in contents ==> key !in underlying.contents || underlying.contents[key].None?)
+  }
+
+  predicate UnderlyingInv<V>(self: LinearHashMap<V>, underlying: FixedSizeLinearHashMap<V>)
+  {
+    && |self.contents| == self.count as nat
+    && UnderlyingContentsMatchesContents(underlying, self.contents)
+    && FixedSizeInv(underlying)
+    && MapFromStorage(toItems(underlying.storage)) == self.contents
+  }
+
+  lemma UnderlyingInvImpliesMapFromStorageMatchesContents<V>(underlying: FixedSizeLinearHashMap<V>, contents: map<uint64, V>)
+  requires UnderlyingContentsMatchesContents(underlying, contents)
+  requires FixedSizeInv(underlying)
+  ensures MapFromStorage(toItems(underlying.storage)) == contents
+  {
+    var mapFromStorage := MapFromStorage(toItems(underlying.storage));
+    CantEquivocateMapFromStorageKey(underlying);
+    MapFromStorageProperties(toItems(underlying.storage), mapFromStorage);
+    assert MapFromStorage(toItems(underlying.storage)) == contents;
+  }
+
+  predicate Inv0<V>(self: LinearHashMap<V>) { Inv(self) }
+
+  protected predicate Inv<V>(self: LinearHashMap<V>)
+  ensures Inv(self) ==> |self.contents| == self.count as nat
+  ensures Inv(self) ==> UnderlyingInv(self, self.underlying)
+  {
+    && UnderlyingInv(self, self.underlying)
+    && MapFromStorage(toItems(self.underlying.storage)) == self.contents
+    && |self.contents| == self.count as nat
+    && (self.count as nat) <= 0x1_0000_0000_0000_0000 / 8
+  }
+
+  lemma CountBound<V>(self: LinearHashMap<V>)
+  requires Inv(self)
+  ensures self.count as int <= 0x1_0000_0000_0000_0000 / 8
+  {
+  }
+
+  lemma RevealProtectedInv<V>(self: LinearHashMap<V>)
+    requires Inv(self)
+    ensures (
+      && UnderlyingInv(self, self.underlying)
+      && MapFromStorage(toItems(self.underlying.storage)) == self.contents
+      && |self.contents| == self.count as nat)
+  {
+  }
+
+  predicate IsConstructor<V>(self: LinearHashMap<V>, size: uint64)
+  requires 128 <= size
+  {
+    && Inv(self)
+    && self.contents == map[]
+  }
+
+  method Constructor<V>(size: uint64) returns (linear self: LinearHashMap<V>)
+  requires 128 <= size
+  ensures IsConstructor(self, size)
+  {
+    linear var fixed := ConstructorFromSize(size);
+    self := LinearHashMap(fixed, 0, map[]);
+
+    assert forall slot :: ValidSlot(|self.underlying.storage|, slot) ==> !self.underlying.storage[slot.slot].Entry?;
+    UnderlyingInvImpliesMapFromStorageMatchesContents(self.underlying, self.contents);
+    assert MapFromStorage(toItems(self.underlying.storage)) == self.contents;
+  }
+
+  lemma LemmaEntryKeyInContents<V>(self: LinearHashMap<V>, i: uint64)
+  requires Inv(self)
+  requires 0 <= i as int < |self.underlying.storage|
+  requires self.underlying.storage[i as nat].Entry?
+  ensures self.underlying.storage[i as nat].key in self.contents
+  {
+    assert EntryInSlotMatchesContents(toItems(self.underlying.storage), Slot(i as nat), self.underlying.contents); // trigger
+  }
+
+  predicate IsRealloc<V>(self: LinearHashMap<V>, self': LinearHashMap<V>)
+  requires Inv(self)
+  requires self.count as nat < 0x1_0000_0000_0000_0000 / 8
+  {
+    && self'.contents == self.contents
+    && self'.underlying.count as nat < |self'.underlying.storage| - 2
+    && Inv(self')
+  }
+
+  method Realloc<V>(linear inout self: LinearHashMap<V>)
+  requires Inv(old_self)
+  requires old_self.count as nat < 0x1_0000_0000_0000_0000 / 8
+  ensures IsRealloc(old_self, self)
+  {
+    var newSize: uint64 := (128 + self.count) * 4;
+    linear var newUnderlying := ConstructorFromSize(newSize);
+
+    ghost var transferredContents := map[];
+    ghost var transfers := toItems(self.underlying.storage);
+    CantEquivocateMapFromStorageKey(self.underlying);
+
+    var i := 0 as uint64;
+    var size := lseq_length_as_uint64(self.underlying.storage);
+
+    while i < size
+      invariant i <= size
+      invariant size as nat == |self.underlying.storage|
+      invariant self.count as nat == |self.contents|
+      invariant |newUnderlying.storage| == newSize as nat
+
+      invariant transferredContents.Keys <= self.contents.Keys
+      invariant newUnderlying.count as nat == |transferredContents|
+      invariant newUnderlying.count as nat < |newUnderlying.storage| - 2
+      invariant (forall key :: key in newUnderlying.contents ==> 
+        EntryExistsInElements(transfers, i, key))
+
+      invariant FixedSizeInv(newUnderlying)
+      invariant UnderlyingContentsMatchesContents(newUnderlying, transferredContents)
+      invariant toItems(self.underlying.storage)[i..] == transfers[i..]
+      invariant MapFromStorage(transfers[..i]) == transferredContents
+      invariant MapFromStorage(transfers) == self.contents
+
+      invariant (forall j | i as nat <= j < size as nat :: lseq_has(self.underlying.storage)[j])
+      invariant (forall j | 0 <= j < i as nat :: !lseq_has(self.underlying.storage)[j])
+    {
+      assert i < size;
+      assert Last(transfers[..i+1]) == transfers[i];
+      assert transfers[..i] == DropLast(transfers[..i+1]);
+
+      linear var item := lseq_take_inout(inout self.underlying.storage, i);
+      if item.Entry? {
+        ElementsEntryInMap(transfers, item.toItem());
+        if item.key in newUnderlying.contents {
+          var j:uint64 :| (
+              && 0 <= j < i
+              && ValidSlot(|transfers|, Slot(j as int))
+              && transfers[Slot(j as int).slot].Entry?
+              && transfers[Slot(j as int).slot].key == item.key);
+          assert ValidSlot(|transfers|, Slot(i as nat));
+          assert false;
+        }
+        assert item.key !in newUnderlying.contents;
+
+        assert transferredContents.Keys <= self.contents.Keys;
+        SetInclusionImpliesSmallerCardinality(transferredContents.Keys, self.contents.Keys);
+        assert |transferredContents.Keys| <= |self.contents.Keys|;
+        assert |transferredContents| <= |self.contents|;
+        assert newUnderlying.count as nat < |newUnderlying.storage| - 1;
+
+        // ------ Mutation ------
+        transferredContents := transferredContents[item.key := item.value];
+        linear var replaced := FixedSizeInsertEntry(inout newUnderlying, item);
+        // ----------------------
+        linear match replaced { case lNone() => }
+        assert ValidSlot(|transfers|, Slot(i as nat));
+        assert FixedSizeInv(newUnderlying);
+      } else {
+        item.FreeNonEntry();
+      }
+      assert newUnderlying.count as nat < |newUnderlying.storage| - 2;
+      i := i + 1;
+    }
+
+    assert transfers[..i] == transfers;
+    assert UnderlyingContentsMatchesContents(newUnderlying, transferredContents);
+    assert UnderlyingContentsMatchesContents(newUnderlying, self.contents);
+    UnderlyingInvImpliesMapFromStorageMatchesContents(newUnderlying, self.contents);
+
+    linear var oldUnderlying := Replace(inout self.underlying, newUnderlying);
+    linear var FixedSizeLinearHashMap(oldstorage, _, _) := oldUnderlying;
+    lseq_free(oldstorage);
+  }
+
+  method Insert<V>(linear inout self: LinearHashMap, key: uint64, linear value: V) 
+  returns (linear replaced: lOption<V>)
+  requires Inv(old_self)
+  requires old_self.count as nat < 0x1_0000_0000_0000_0000 / 8
+  ensures
+    && Inv(self)
+    && self.contents == old_self.contents[key := value]
+    && self.count as nat == old_self.count as nat + (if replaced.lSome? then 0 else 1)
+    && (replaced.lSome? ==> MapsTo(old_self.contents, key, replaced.value))
+    && (replaced.lNone? ==> key !in old_self.contents)
+  {
+    var len := lseq_length_as_uint64(self.underlying.storage);
+    if len / 2 <= self.underlying.count {
+      Realloc(inout self);
+    }
+    // --------------
+
+    // -- mutation --
+    replaced := FixedSizeInsert(inout self.underlying, key, value);
+    inout ghost self.contents := self.contents[key := value];
+    if replaced.lNone? {
+      inout self.count := self.count + 1;
+    }
+    // --------------
+
+    UnderlyingInvImpliesMapFromStorageMatchesContents(self.underlying, self.contents);
+  }
+
+  method Remove<V>(linear inout self: LinearHashMap, key: uint64) 
+  returns (linear removed: lOption<V>)
+  requires Inv(old_self)
+  ensures Inv(self)
+  ensures removed.lSome? ==>
+      key in old_self.contents && old_self.contents[key] == removed.value
+  ensures removed.lNone? ==> key !in old_self.contents
+  ensures (self.contents == if key in old_self.contents
+      then map k | k in old_self.contents && k != key :: old_self.contents[k]
+      else old_self.contents)
+  {
+    // -- mutation --
+    removed := FixedSizeRemove(inout self.underlying, key);
+    inout ghost self.contents := map k | k in self.contents && k != key :: self.contents[k];
+    if removed.lSome? {
+      inout self.count := self.count - 1;
+    }
+    // -------------- 
+
+    UnderlyingInvImpliesMapFromStorageMatchesContents(self.underlying, self.contents); 
+    assert self.count as nat == |self.contents| by {
+      if removed.lSome? {
+        assert key in old_self.contents;
+        assert self.contents.Keys <= old_self.contents.Keys;
+        assert |old_self.contents| == self.count as nat + 1;
+        assert |old_self.contents.Keys| == self.count as nat + 1;
+        assert |old_self.contents.Keys - {key}| == |old_self.contents.Keys| - |{key}|;
+        assert old_self.contents.Keys - {key} == self.contents.Keys;
+        assert |self.contents| == |old_self.contents| - 1;
+        assert |self.contents| == self.count as nat;
+      } else {
+        assert key !in old_self.contents;
+        assert self.contents == old_self.contents;
+        assert |self.contents| == self.count as nat;
+      }
+    }
+  }
+
+  method Get<V>(shared self: LinearHashMap, key: uint64) returns (shared result: V)
+  requires Inv(self)
+  requires key in self.underlying.contents && self.underlying.contents[key].Some?
+  ensures key in self.contents && result == self.contents[key]
+  {
+    result := FixedSizeGet(self.underlying, key);
+  }
+}
