lib/DataStructures/LinearMutableMapBase.i.dfy
@@ -1,0 +1,460 @@
+include "../Lang/NativeTypes.s.dfy"
+include "../Lang/System/Arithmetic.s.dfy"
+include "../Base/SetBijectivity.i.dfy"
+include "../Base/sequences.i.dfy"
+include "../Base/Option.s.dfy"
+
+module LinearMutableMapBase {
+  import opened NativeTypes
+  import opened SetBijectivity
+  import opened NativeArithmetic
+  import opened Options
+  import opened Sequences
+
+  function method {:opaque} lshift(a: uint64, b: uint32) : uint64
+  requires 0 <= b < 64
+  {
+    ((a as bv64) << b) as uint64
+  }
+
+  function method {:opaque} rshift(a: uint64, b: uint32) : uint64
+  requires 0 <= b < 64
+  {
+    ((a as bv64) >> b) as uint64
+  }
+
+  function method {:opaque} bitnot(a: uint64) : uint64
+  {
+    ((a as bv64) ^ 0xffff_ffff_ffff_ffff) as uint64
+  }
+
+  function method {:opaque} bitxor(a: uint64, b: uint64) : uint64
+  {
+    ((a as bv64) ^ (b as bv64)) as uint64
+  }
+
+  function method {:opaque} hash64(k: uint64): uint64
+  {
+    var k0 := u64add(bitnot(k), lshift(k, 21));
+    var k1 := bitxor(k0, rshift(k0, 24));
+    var k2 := u64add(u64add(k1, lshift(k1, 3)), lshift(k1, 8));
+    var k3 := bitxor(k2, rshift(k2, 14));
+    var k4 := u64add(u64add(k3, lshift(k3, 2)), lshift(k3, 4));
+    var k5 := bitxor(k4, rshift(k4, 28));
+    var k6 := u64add(k5, lshift(k5, 31));
+
+    k6
+  }
+
+  datatype Slot = Slot(ghost slot: nat)
+  datatype Item<V> = Empty | Entry(key: uint64, value: V) | Tombstone(key: uint64)
+
+  predicate ValidSlot(elementsLength: nat, slot: Slot)
+  {
+    slot.slot < elementsLength
+  }
+
+  predicate ValidElements<V>(elements: seq<Item<V>>)
+  {
+    && 0 < |elements| < 0x1_0000_0000_0000_0000
+  }
+
+  function SlotForKey(elementsLength: nat, key: uint64): (result: Slot)
+  requires 0 < elementsLength
+  ensures ValidSlot(elementsLength, result)
+  {
+    var h := hash64(key);
+    Slot((h as nat) % elementsLength)
+  }
+
+  function SlotSuccessor(elementsLength: nat, slot: Slot): (nextSlot: Slot)
+  requires ValidSlot(elementsLength, slot)
+  ensures ValidSlot(elementsLength, nextSlot)
+  {
+    Slot(if slot.slot == elementsLength - 1 then
+      0
+    else
+      slot.slot + 1)
+  }
+
+  function KthSlotSuccessor(elementsLength: nat, slot: Slot, k: nat): (nextSlot: Slot)
+    requires k >= 0
+    requires ValidSlot(elementsLength, slot)
+    ensures ValidSlot(elementsLength, nextSlot)
+  {
+    if k == 0 then
+      slot
+    else
+      SlotSuccessor(elementsLength, KthSlotSuccessor(elementsLength, slot, k - 1))
+  }
+
+  // KthSlotSuccessorWrapsAround
+  //
+  //   0 - - - - - - - - - - -   length = 12
+  //                 @           slot = 7
+  //                 | > > *     k = 3; (slot + k) mod length is slot 10 == 7 + 3
+  //
+  //   0 - - - - - - - - - - -   length = 12
+  //                 @           slot = 7
+  //                 | > > > >   k = 8
+  //   > > > *                   (slot + k) mod length is slot 3 == 8 - (12 - 7) == 8 - 5 == 3
+  //
+  lemma KthSlotSuccessorWrapsAround(elementsLength: nat, slot: Slot, k: nat)
+    requires 0 <= k < elementsLength
+    requires ValidSlot(elementsLength, slot)
+    ensures if k < (elementsLength-slot.slot) then
+          KthSlotSuccessor(elementsLength, slot, k).slot == slot.slot + k
+        else
+          KthSlotSuccessor(elementsLength, slot, k).slot == k - (elementsLength - slot.slot)
+    decreases k
+  {
+    /* (doc)
+      var elementsInRightSlice := elementsLength - slot.slot;
+      if k < elementsInRightSlice {
+      } else {
+        var firstSlot := KthSlotSuccessor(elementsLength, slot, elementsInRightSlice);
+        var idx: nat := k - elementsInRightSlice;
+        KthSlotSuccessorWrapsAround(elementsLength, firstSlot, idx);
+      }
+    */
+  }
+
+  predicate SlotIsEmpty<V>(elements: seq<Item<V>>, slot: Slot) // hide trigger
+  requires ValidSlot(|elements|, slot)
+  {
+    elements[slot.slot].Empty?
+  }
+
+  predicate SlotIsEntry<V>(elements: seq<Item<V>>, slot: Slot) // hide trigger
+  requires ValidSlot(|elements|, slot)
+  {
+    elements[slot.slot].Entry?
+  }
+
+  predicate SlotIsTombstone<V>(elements: seq<Item<V>>, slot: Slot) // hide trigger
+  requires ValidSlot(|elements|, slot)
+  {
+    elements[slot.slot].Tombstone?
+  }
+
+  predicate FilledWithOtherKey<V>(elements: seq<Item<V>>, slot: Slot, excludingKey: uint64)
+    requires ValidElements(elements)
+    requires ValidSlot(|elements|, slot)
+  {
+    || (SlotIsTombstone(elements, slot) && elements[slot.slot].key != excludingKey)
+    || (SlotIsEntry(elements, slot) && elements[slot.slot].key != excludingKey)
+  }
+
+  predicate FilledWithOtherKeys<V>(elements: seq<Item<V>>, start: Slot, count: nat, excludingKey: uint64)
+    requires ValidElements(elements)
+    requires ValidSlot(|elements|, start)
+  {
+    && (forall offset: nat :: offset < count ==>
+      FilledWithOtherKey(elements, KthSlotSuccessor(|elements|, start, offset), excludingKey))
+  }
+
+  predicate FilledWithKey<V>(elements: seq<Item<V>>, slot: Slot, key: uint64)
+    requires ValidElements(elements)
+    requires ValidSlot(|elements|, slot)
+  {
+    (SlotIsEntry(elements, slot) || SlotIsTombstone(elements, slot)) && elements[slot.slot].key == key
+  }
+
+  predicate FilledWithEntryKey<V>(elements: seq<Item<V>>, slot: Slot, key: uint64)
+    requires ValidElements(elements)
+    requires ValidSlot(|elements|, slot)
+  {
+    && SlotIsEntry(elements, slot)
+    && elements[slot.slot].key == key
+  }
+
+  predicate SlotExplainsKey<V>(elements: seq<Item<V>>, skips: nat, key: uint64)
+  requires ValidElements(elements)
+  {
+    var foundSlot := KthSlotSuccessor(|elements|, SlotForKey(|elements|, key), skips);
+    && ValidSlot(|elements|, foundSlot)
+    && FilledWithOtherKeys(elements, SlotForKey(|elements|, key), skips, key)
+    && FilledWithKey(elements, foundSlot, key)
+  }
+
+  predicate {:opaque} SomeSkipCountExplainsKey<V>(elements: seq<Item<V>>, key: uint64)
+  requires ValidElements(elements)
+  {
+    exists skips :: SlotExplainsKey(elements, skips, key)
+  }
+
+  // hide forall trigger
+  predicate TwoNonEmptyValidSlotsWithSameKey<V>(elements: seq<Item<V>>, slot1: Slot, slot2: Slot)
+  requires ValidElements(elements)
+  {
+    && ValidSlot(|elements|, slot1)
+    && ValidSlot(|elements|, slot2)
+    && (SlotIsEntry(elements, slot1) || SlotIsTombstone(elements, slot1))
+    && (SlotIsEntry(elements, slot2) || SlotIsTombstone(elements, slot2))
+    && elements[slot1.slot].key == elements[slot2.slot].key
+  }
+
+  // hide forall trigger
+  predicate SameSlot(elementsLength: nat, slot1: Slot, slot2: Slot)
+  requires ValidSlot(elementsLength, slot1)
+  requires ValidSlot(elementsLength, slot2)
+  {
+    slot1 == slot2
+  }
+
+  predicate CantEquivocateStorageKey<V>(elements: seq<Item<V>>)
+    requires ValidElements(elements)
+  {
+    forall slot1, slot2 :: TwoNonEmptyValidSlotsWithSameKey(elements, slot1, slot2)
+        ==> SameSlot(|elements|, slot1, slot2)
+  }
+
+  predicate KeyInSlotIsInContents<V>(elements: seq<Item<V>>, contents: map<uint64, Option<V>>, slot: Slot)
+  requires ValidSlot(|elements|, slot)
+  requires SlotIsEntry(elements, slot) || SlotIsTombstone(elements, slot)
+  {
+    && var key := elements[slot.slot].key;
+    && key in contents
+  }
+
+  predicate SeqMatchesContentKeys<V>(elements: seq<Item<V>>, contents: map<uint64, Option<V>>)
+  requires ValidElements(elements)
+  {
+    && (forall key :: key in contents ==> exists skips :: SlotExplainsKey(elements, skips, key))
+    && (forall slot :: ValidSlot(|elements|, slot) && (SlotIsEntry(elements, slot) || SlotIsTombstone(elements, slot))
+        ==> KeyInSlotIsInContents(elements, contents, slot))
+    && CantEquivocateStorageKey(elements)
+  }
+
+  predicate EntryInSlotMatchesContents<V>(elements: seq<Item<V>>, slot: Slot, contents: map<uint64, Option<V>>) // hide triggers
+  requires ValidSlot(|elements|, slot)
+  requires SlotIsEntry(elements, slot)
+  {
+    && var item := elements[slot.slot];
+    && item.key in contents
+    && contents[item.key] == Some(item.value)
+  }
+
+  predicate TombstoneInSlotMatchesContents<V>(elements: seq<Item<V>>, slot: Slot, contents: map<uint64, Option<V>>) // hide triggers
+  requires ValidSlot(|elements|, slot)
+  requires SlotIsTombstone(elements, slot)
+  {
+    && var item := elements[slot.slot];
+    && item.key in contents
+    && contents[item.key].None?
+  }
+
+  predicate EntriesMatchContentValue<V>(elements: seq<Item<V>>, contents: map<uint64, Option<V>>) // hide triggers
+  requires ValidElements(elements)
+  {
+    forall slot :: ValidSlot(|elements|, slot) && SlotIsEntry(elements, slot)
+        ==> EntryInSlotMatchesContents(elements, slot, contents)
+  }
+
+  predicate TombstonesMatchContentValue<V>(elements: seq<Item<V>>, contents: map<uint64, Option<V>>) // hide triggers
+  requires ValidElements(elements)
+  {
+    forall slot :: ValidSlot(|elements|, slot) && SlotIsTombstone(elements, slot)
+        ==> TombstoneInSlotMatchesContents(elements, slot, contents)
+  }
+
+    function IndexSetThrough<V>(elements: seq<Item<V>>, through: nat): set<int>
+    requires through <= |elements|
+  {
+    set i | 0 <= i < through && (elements[i].Entry? || elements[i].Tombstone?)
+  }
+
+  function IndexSet<V>(elements: seq<Item<V>>): set<int>
+  {
+    IndexSetThrough(elements, |elements|)
+  }
+
+  function Count1<V>(item: Item<V>): nat
+  {
+    if item.Entry? || item.Tombstone? then 1 else 0
+  }
+
+  function CountFilled<V>(view: seq<Item<V>>): (result: nat)
+  {
+    if |view| == 0 then
+      0
+    else
+      CountFilled(view[1..]) + Count1(view[0])
+  }
+
+  lemma CountFilledMatchesIndexSet<V>(elements: seq<Item<V>>)
+  ensures CountFilled(elements) == |IndexSet(elements)|
+  {
+    var i: nat := 0;
+    while i < |elements|
+      invariant i <= |elements|
+      invariant |IndexSetThrough(elements, i)| == CountFilled(elements[..i])
+    {
+      var j := i + 1;
+      CountFilledAdditive(elements[..i], [elements[i]]);
+      assert elements[..i] + [elements[i]] == elements[..j]; // observe
+      if elements[i].Entry? || elements[i].Tombstone? {
+        assert IndexSetThrough(elements, j) == IndexSetThrough(elements, i) + {i}; // observe
+      } else {
+        assert IndexSetThrough(elements, j) == IndexSetThrough(elements, i); // observe
+      }
+      i := j;
+    }
+    assert elements[..i] == elements; // observe
+  }
+
+  lemma IndexSetMatchesContents<V>(elements: seq<Item<V>>, contents: map<uint64, Option<V>>)
+  requires ValidElements(elements)
+  requires SeqMatchesContentKeys(elements, contents)
+  ensures |IndexSet(elements)| == |contents.Keys|
+  {
+    var relation := iset i | i in IndexSet(elements) :: (i, elements[i].key);
+    var setA := IndexSet(elements);
+    var setB := contents.Keys;
+    assert forall a | a in setA
+      :: SlotIsEntry(elements, Slot(a)) || SlotIsTombstone(elements, Slot(a)); // observe
+    assert forall a1, a2, b | a1 in setA && a2 in setA && b in setB && (a1, b) in relation && (a2, b) in relation
+      :: SameSlot(|elements|, Slot(a1), Slot(a2)); // observe
+    BijectivityImpliesEqualCardinality(IndexSet(elements), contents.Keys, relation);
+  }
+
+  lemma CountFilledAdditive<V>(a: seq<Item<V>>, b: seq<Item<V>>)
+  ensures CountFilled(a + b) == CountFilled(a) + CountFilled(b)
+  {
+    if |a| == 0 {
+      assert a + b == b; // observe
+    } else {
+      assert (a + b)[1..] == a[1..] + b; // observe
+    }
+  }
+
+  function View<V>(elements: seq<Item<V>>, start: nat): (result: seq<Item<V>>)
+  requires start < |elements|
+  ensures |result| == |elements|
+  {
+    elements[start..] + elements[..start]
+  }
+
+  lemma ViewsHaveConsistentCounts<V>(a: seq<Item<V>>, b: seq<Item<V>>, delta: nat)
+  requires delta < |a|
+  requires b == View(a, delta)
+  ensures CountFilled(a) == CountFilled(b)
+  {
+    var n := |a|;
+    assert a == a[..delta] + a[delta..]; // observe
+    CountFilledAdditive(a[..delta], a[delta..]);
+    CountFilledAdditive(b[..n-delta], b[n-delta..]);
+    assert b == b[..n-delta] + b[n-delta..]; // observe
+  }
+
+  function Uint64SlotSuccessor(elementsLength: nat, slot: uint64): (nextSlot: uint64)
+  requires elementsLength < 0x1_0000_0000_0000_0000
+  requires ValidSlot(elementsLength, Slot(slot as nat))
+  ensures ValidSlot(elementsLength, Slot(nextSlot as nat))
+  ensures Slot(nextSlot as nat) == SlotSuccessor(elementsLength, Slot(slot as nat))
+  {
+    Uint64SlotSuccessorUint64(elementsLength as uint64, slot)
+  }
+
+  // TODO rename
+  function method Uint64SlotSuccessorUint64(elementsLength: uint64, slot: uint64): (nextSlot: uint64)
+  requires ValidSlot(elementsLength as nat, Slot(slot as nat))
+  ensures ValidSlot(elementsLength as nat, Slot(nextSlot as nat))
+  ensures Slot(nextSlot as nat) == SlotSuccessor(elementsLength as nat, Slot(slot as nat))
+  {
+    if slot == (elementsLength as uint64) - 1 then
+      0
+    else
+      slot + 1
+  }
+
+  function MapFromStorage<V>(elements: seq<Item<V>>): (result: map<uint64, V>)
+  {
+    if |elements| == 0 then
+      map[]
+    else
+      var item := Last(elements);
+      var dropLastMap := MapFromStorage(DropLast(elements));
+      if item.Entry? then
+        dropLastMap[item.key := item.value]
+      else
+        dropLastMap
+  }
+
+  // TODO(jonh): This should just be CantEquivocateStorageKey, because (a) it's
+  // the same and (b) this expression is a trigger nest.  But doing so will
+  // involve cleaning up the proofs that break when we re-hide the definition.
+  predicate CantEquivocate<V>(elements: seq<Item<V>>)
+  {
+    forall slot1, slot2 :: ValidSlot(|elements|, slot1) && ValidSlot(|elements|, slot2) &&
+        elements[slot1.slot].Entry? && elements[slot2.slot].Entry? &&
+        elements[slot1.slot].key == elements[slot2.slot].key ==> slot1 == slot2
+  }
+
+  lemma MapFromStorageProperties<V>(elements: seq<Item<V>>, result: map<uint64, V>)
+  requires CantEquivocate(elements)
+  requires MapFromStorage(elements) == result
+  ensures forall slot :: ValidSlot(|elements|, slot) && elements[slot.slot].Entry? ==>
+    && var item := elements[slot.slot];
+    && item.key in result && result[item.key] == item.value
+  ensures forall key :: key in result ==>
+    exists slot :: ValidSlot(|elements|, slot) && elements[slot.slot] == Entry(key, result[key])
+  ensures forall key :: key !in result ==>
+    forall slot :: ValidSlot(|elements|, slot) && elements[slot.slot].Entry?
+      ==> elements[slot.slot].key != key
+  {
+    if |elements| == 0 {
+    } else if Last(elements).Entry? {
+      var item := Last(elements);
+      assert elements == DropLast(elements) + [Last(elements)];
+      var dropLastMap := MapFromStorage(DropLast(elements));
+      MapFromStorageProperties(DropLast(elements), dropLastMap);
+
+      forall slot | ValidSlot(|elements|, slot) && elements[slot.slot].Entry?
+      ensures && var item := elements[slot.slot];
+              && item.key in result && result[item.key] == item.value
+      {
+        var slotItem := elements[slot.slot];
+        if item.key == elements[slot.slot].key {
+          if slot.slot == |elements| - 1 {
+            assert slotItem.key in result && result[slotItem.key] == slotItem.value;
+          } else {
+            var slot := Slot(|elements| - 1);
+            assert ValidSlot(|elements|, slot);
+            assert false;
+          }
+        } else {
+          assert slotItem.key in result && result[slotItem.key] == slotItem.value;
+        }
+      }
+      forall key | key in result
+      ensures exists slot :: ValidSlot(|elements|, slot) && elements[slot.slot] == Entry(key, result[key])
+      {
+        if key == item.key {
+          var slot := Slot(|elements| - 1);
+          assert ValidSlot(|elements|, slot);
+          assert elements[slot.slot] == Entry(key, result[key]);
+        } else {
+          assert exists slot :: ValidSlot(|elements|, slot) && elements[slot.slot] == Entry(key, result[key]);
+        }
+      }
+    } else {
+    }
+  }
+
+  predicate EntryExistsInElements<V>(elements: seq<Item<V>>, i: uint64, key: uint64)
+  requires i as int <= |elements|
+  requires ValidElements(elements)
+  {
+    && (exists slot: Slot :: ( && slot.slot < i as int
+        && ValidSlot(|elements|, slot)
+        && FilledWithEntryKey(elements, slot, key)))
+  }
+
+  lemma ElementsEntryInMap<V>(elements: seq<Item<V>>, item: Item<V>)
+  requires item.Entry?
+  requires item in elements
+  ensures item.key in MapFromStorage(elements)
+  {
+  }
+}
